Add coercion instead of notation for eval_map.

TotalMap.v
@@ -32,17 +32,17 @@ Fixpoint eval_map {A: Type} (m: @total_map A) (x: string) :=
   | TUpdate m' x' v => if x' =? x then v else eval_map m' x
   end.
 
-(* Notation for evaluation *)
-Notation "m [| x |] " := (eval_map m x) (at level 65).
+(* Coercion for evaluation *)
+Coercion eval_map : total_map >-> Funclass.
 
 Lemma t_apply_empty : forall (A : Type) (x : string) (v : A),
-    (_ !-> v)[|x|] = v.
+    (_ !-> v) x = v.
 Proof.
   by [].
 Qed.
 
 Lemma t_update_eq : forall (A : Type) (m : total_map A) (x: string) (v: A),
-    (x !-> v ; m)[|x|] = v.
+    (x !-> v ; m) x = v.
 Proof.
   move => A m x v /=.
   by rewrite eqb_refl.
@@ -50,7 +50,7 @@ Qed.
 
 Theorem t_update_neq : forall (A : Type) (m : total_map A) (x1 x2: string) (v: A),
     x1 <> x2 ->
-    (x1 !-> v ; m)[|x2|] = m[|x2|].
+    (x1 !-> v ; m) x2 = m x2.
 Proof.
   by move => A m x1 x2 v /eqb_neq /= ->.
 Qed.
@@ -94,7 +94,7 @@ Fixpoint pointwise_un_op {A B: Type} (m: total_map A) (f: A -> B) :=
   end.
 
 Theorem pointwise_un_op_spec {A B: Type} :
-  forall m (f: A -> B) v, (pointwise_un_op m f)[|v|] = f (m[|v|]).
+  forall m (f: A -> B) v, (pointwise_un_op m f) v = f (m v).
 Proof.
   elim => [// | m Hind v x f v' /=].
   rewrite Hind.
@@ -109,7 +109,7 @@ Fixpoint pointwise_bin_op_aux {A B C: Type} (m1: total_map A) (x2: B) (f: A -> B
   end.
 
 Lemma pointwise_bin_op_aux_spec {A B C: Type} :
-  forall m1 x2 (f: A -> B -> C) s, (pointwise_bin_op_aux m1 x2 f)[|s|] = f (m1[|s|]) x2.
+  forall m1 x2 (f: A -> B -> C) s, (pointwise_bin_op_aux m1 x2 f) s = f (m1 s) x2.
 Proof.
   elim => [// | m H s x1 x2 f s' /=].
   rewrite H.
@@ -120,11 +120,11 @@ Fixpoint pointwise_bin_op {A B C: Type} (m1: total_map A) (m2: total_map B) (f: 
   match m2 with
   | TEmpty x2 => pointwise_bin_op_aux m1 x2 f
   | TUpdate m2' v x2 => let new_m := pointwise_bin_op m1 m2' f in
-                       (v !-> (f (m1[|v|]) x2); new_m)
+                       (v !-> (f (m1 v) x2); new_m)
   end.
 
 Theorem pointwise_bin_op_spec {A B C: Type} :
-  forall m1 m2 (f: A -> B -> C) x, (pointwise_bin_op m1 m2 f)[|x|] = f (m1[|x|]) (m2[|x|]).
+  forall m1 m2 (f: A -> B -> C) x, (pointwise_bin_op m1 m2 f) x = f (m1 x) (m2 x).
 Proof.
   move => m1 m2.
   elim: m2 m1 => [v m1 f x | m Hind x v m1 f x0 /=].
@@ -236,7 +236,7 @@ Fixpoint forall_bin_op_aux {A: Type} (m1: total_map A) (x2: A) (f: A -> A -> boo
 
 Lemma forall_bin_op_aux_spec {A: Type} :
   forall m1 (x2: A) f seen, forall_bin_op_aux m1 x2 f seen <->
-                       (forall v, not (List.In v seen) -> f (m1[|v|]) x2).
+                       (forall v, not (List.In v seen) -> f (m1 v) x2).
 Proof.
   elim => [v x2 f seen /= | m Hind v x1 x2 f seen /=].
     by split => [// | H]; apply (H (construct_not_in_list seen)), construct_not_in_list_spec.
@@ -270,12 +270,12 @@ Fixpoint forall_bin_op_fix {A: Type} (m1 m2: total_map A) (f: A -> A -> bool) (s
     if list_string_in seen v then
       forall_bin_op_fix m1 m2' f seen
     else
-      f (m1[|v|]) x2 && forall_bin_op_fix m1 m2' f (v::seen)
+      f (m1 v) x2 && forall_bin_op_fix m1 m2' f (v::seen)
   end.
 
 Lemma forall_bin_op_fix_spec {A: Type} :
   forall (m1 m2: @total_map A) f seen, forall_bin_op_fix m1 m2 f seen <->
-                                  forall v, not (List.In v seen) -> f (m1[|v|]) (m2[|v|]).
+                                  forall v, not (List.In v seen) -> f (m1 v) (m2 v).
 Proof.
   move => m1 m2; move: m2 m1.
   elim => [m1 m2 f seen /= | m2 Hind v x1 m1 f seen /=].
@@ -307,7 +307,7 @@ Definition forall_bin_op {A: Type} (m1 m2: total_map A) (f: A -> A -> bool) :=
   forall_bin_op_fix m1 m2 f nil.
 
 Theorem forall_bin_op_spec {A: Type} :
-  forall (m1 m2: @total_map A) f, forall_bin_op m1 m2 f <-> forall v, f (m1[|v|]) (m2[|v|]).
+  forall (m1 m2: @total_map A) f, forall_bin_op m1 m2 f <-> forall v, f (m1 v) (m2 v).
 Proof.
   move => m1 m2 f.
   unfold forall_bin_op.
